src/Knapsack/Specification/InputData.dfy
@@ -2,7 +2,7 @@ include "ItemData.dfy"
 
 datatype InputData = InputData(items: seq<ItemData>, maxWeight: real) {
   ghost predicate Valid() {
-    (forall i | 0 <= i < |items| :: items[i].Valid()) &&
-    maxWeight >= 0.0
+    && (forall i | 0 <= i < |items| :: items[i].Valid())
+    && maxWeight >= 0.0
   }
 }
